<?xml version="1.0" encoding="UTF-8"?> 

<!-- ============================================================== --> 
<!--        G e o g r a p h y                                       --> 
<!--        M a r k u p                                             --> 
<!--        L a n g u a g e                                         --> 
<!--                                                                --> 
<!--        ( G M L )                                               --> 
<!--                                                                --> 
<!--        R D F    S c h e m a    D e f i n i t i o n s           --> 
<!--                                                                --> 
<!--  Copyright (c) 2000 Open Geospatial Consortium.                --> 
<!-- ============================================================== --> 

<rdf:RDF xml:lang="en"  
   xmlns:rdf="http://www.w3.org/1999/02/22-rdf-syntax-ns#" 
   xmlns:rdfs="http://www.w3.org/TR/1999/PR-rdf-schema-19990303#"> 

<!--======================================================================================--> 
<!--===  This section describes the abstract classes and properties for core GML =========--> 
<!--======================================================================================--> 

   <rdfs:Class rdf:ID="Geometry"> 
      <rdfs:comment> 
Geometry is the root class of the hierarchy. Geometry is an abstract (non-instantiable) class. 
All instantiable geometry classes referenced in this specification are defined so that valid
instances of a geometry class are topologically closed (i.e. all defined  geometries include
their boundary). 
      </rdfs:comment> 
   </rdfs:Class> 

   <rdfs:Class rdf:ID="Feature"> 
      <rdfs:comment> 
A Feature is a Property List, some of whose properties are of type geometry. Specific classes
of geographic feature are created by subtyping from the GML Feature class in the application
namespace. 
      </rdfs:comment> 
   </rdfs:Class> 

   <rdfs:Class rdf:ID="GeometryCollection"> 
      <rdfs:subClassOf rdf:resource="#Geometry"/> 
      <rdfs:subClassOf
rdf:resource="http://www.w3.org/TR/1999/PR-rdf-schema-19990303#Container"/> 
      <rdfs:comment> 
A GeometryCollection is a geometry that is a collection of 1 or more geometries. All the
elements in a GeometryCollection must be in the same Spatial Reference. This is also the
Spatial Reference for the GeometryCollection. GeometryCollection places no other constraints on
its elements. Subclasses of GeometryCollection may restrict membership based on dimension and
may also place other constraints on the degree of spatial overlap between elements. 
      </rdfs:comment> 
   </rdfs:Class> 

   <rdfs:Class rdf:ID="Box"> 
      <rdfs:subClassOf rdf:resource="#Geometry"/> 
      <rdfs:comment> 
A rectangular area defined by two points and the four orthogonal geodesic curves defined by
these two points 
      </rdfs:comment> 
   </rdfs:Class> 

   <rdf:Property ID="geometryMember"> 
      <rdfs:range rdf:resource="#Geometry"/> 
      <rdfs:domain rdf:resource="#GeometryCollection"/> 
      <rdfs:comment> 
selects next member in the geometry collection. Plays same role as li tag in rdf 
      </rdfs:comment> 
   </rdf:Property> 

   <rdf:Property ID="geometryProperty"> 
      <rdfs:range rdf:resource="#Geometry"/> 
      <rdfs:domain rdf:resource="#Feature"/> 
      <rdfs:comment> 
Abstract property which is the parent of all geospatial properties.  While OGC provides some
standard geometry properties users can create additional properties by using the subProperty
relationship and deriving from the OGC properties. 
      </rdfs:comment> 
   </rdf:Property> 

   <rdfs:Class rdf:ID="FeatureCollection"> 
      <rdfs:subClassOf rdf:resource="#Feature"/> 
      <rdfs:comment> 
A collection (set) of Features 
      </rdfs:comment> 
   </rdfs:Class> 

   <rdf:Property ID="featureMember"> 
      <rdfs:range rdf:resource="#Feature"/> 
      <rdfs:domain rdf:resource="#FeatureCollection"/> 
      <rdfs:comment> 
Function which returns next Feature in a FeatureCollection 
      </rdfs:comment> 
   </rdf:Property> 

<!--=============================================================================--> 
<!--============== This next section defines common metadata properties =========--> 
<!--=============================================================================--> 

   <rdf:Property ID="name"> 
      <rdfs:range rdf:resource="http://www.w3.org/TR/1999/PR-rdf-schema-19990303#Literal"/> 
      <rdfs:domain rdf:resource="#Feature"/> 
   </rdf:Property> 

   <rdf:Property ID="boundedBy"> 
      <rdfs:range rdf:resource="#Box"/> 
      <rdfs:domain rdf:resource="#Feature"/> 
   </rdf:Property> 

   <rdf:Property ID="description"> 
      <rdfs:range rdf:resource="http://www.w3.org/TR/1999/PR-rdf-schema-19990303#Literal"/> 
      <rdfs:domain rdf:resource="#Feature"/> 
   </rdf:Property> 

   <rdf:Property ID="srsName"> 
      <rdfs:range rdf:resource="http://www.w3.org/TR/1999/PR-rdf-schema-19990303#Literal"/> 
      <rdfs:domain rdf:resource="#Geometry"/> 
   </rdf:Property> 

   <rdf:Property ID="coordinates"> 
      <rdfs:domain rdf:resource="#Curve"/> 
      <rdfs:domain rdf:resource="#Box"/>  
      <rdfs:domain rdf:resource="#Point"/> 
      <rdfs:range  rdf:resource="http://www.w3.org/TR/1999/PR-rdf-schema-19990303#Literal"/> 
   </rdf:Property> 

<!--=============================================================================--> 
<!--=======  This next section defines the GML Geometry Classes =================--> 
<!--=============================================================================--> 

   <rdfs:Class rdf:ID="Point"> 
      <rdfs:subClassOf rdf:resource="#Geometry"/> 
      <rdfs:comment> 
Point geometry class. A Point is a 0-dimensional geometry and represents a single location in
coordinate space. A Point has an x-coordinate value and a y-coordinate value. Note that GML is
more general than the OGC SQL v1.1 specification and does allow Points of 0-4 (or larger)
dimension. The boundary of a Point is the empty set. 
      </rdfs:comment> 
   </rdfs:Class> 

   <rdfs:Class rdf:ID="Curve"> 
      <rdfs:subClassOf rdf:resource="#Geometry"/> 
      <rdfs:comment> 
A Curve is a one-dimensional geometric object usually stored as a sequence of points, with the
subtype of Curve specifying the form of the interpolation between points. This specification
defines only one subclass of Curve, LineString, which uses linear interpolation between
points.  This is the only 1-D Geometry class which appears in the GML DTD. Topologically a
Curve is a one-dimensional geometric object that is the homeomorphic image of a real, closed,
interval D [a, b] {x in R2| a le x le b} under a mapping f:[a,b] --- R2 as defined in [1],
section 3.12.7.2. 

A Curve is simple if it does not pass through the same point twice ([1], section 3.12.7.3). 

A Curve is closed if its start point is equal to its end point. ([1], section 3.12.7.3). 

The boundary of a closed Curve is empty. 

A Curve that is simple and closed is a Ring. 

The boundary of a non-closed Curve consists of its two end points. ([1], section 3.12.3.2). 

A Curve is defined as topologically closed. 
      </rdfs:comment> 
   </rdfs:Class> 

   <rdfs:Class rdf:ID="LineString"> 
      <rdfs:subClassOf rdf:resource="#Curve"/> 
      <rdfs:comment> 
Lines, LineStrings and LinearRings are all Curves. A Line String is a Curve with linear
interpolation between points. Each consecutive pair of points defines a line segment. A Line is
a LineString with exactly 2 points. In GML the points of a LineString are defined by a
coordinate list and are not defined by GML Points. 
      </rdfs:comment> 
   </rdfs:Class> 

   <rdfs:Class rdf:ID="LinearRing"> 
      <rdfs:subClassOf rdf:resource="#Curve"/> 
      <rdfs:comment> 
A LinearRing is a LineString that is both closed and simple.  In GML, the points of a
LinearRing are defined by a coordinate list and are not defined by GML Points. 
      </rdfs:comment> 
   </rdfs:Class> 

   <rdfs:Class rdf:ID="Surface"> 
      <rdfs:subClassOf rdf:resource="#Geometry"/> 
      <rdfs:comment> 
Abstract geometry class for 2D geometries 
      </rdfs:comment> 
   </rdfs:Class> 

   <rdfs:Class rdf:ID="Polygon"> 
      <rdfs:subClassOf rdf:resource="#Surface"/> 
      <rdfs:comment> 
A Polygon is a planar Surface, defined by 1 exterior boundary and 0 or more interior
boundaries. Each interior boundary defines a hole in the Polygon. The assertions for polygons
(the rules that define valid polygons) are: 

1.  Polygons are topologically closed. 

2.  The boundary of a Polygon consists of a set of LinearRings that make up its exterior and
interior boundaries.  Note that these are captured in GML via the eboundaryis and iboundaryis
properties of the Polygon. 

3.  No two rings in the boundary cross, the rings in the boundary of a Polygon may intersect at
a Point but only as a tangent. 

4.  A Polygon may not have cut lines, spikes or punctures: 

5.  The Interior of every Polygon is a connected point set. 

6.  The Exterior of a Polygon with 1 or more holes is not connected. Each hole defines a
connected component of the Exterior. 

In the above assertions, Interior, Closure and Exterior have the standard topological
definitions. The combination of 1 and 3 make a Polygon a Regular Closed point set. Polygons are
simple geometries in accordance with the terminology of the OGC Abstract Specififcation 99-101.

      </rdfs:comment> 
   </rdfs:Class> 

   <rdf:Property ID="outerBoundaryIs"> 
      <rdfs:range rdf:resource="#LinearRing"/> 
      <rdfs:domain rdf:resource="#Polygon"/> 
      <rdfs:comment> 
This property returns the outer boundary of a polygon 
      </rdfs:comment> 
   </rdf:Property> 

   <rdf:Property ID="innerBoundaryIs"> 
      <rdfs:range rdf:resource="#LinearRing"/> 
      <rdfs:domain rdf:resource="#Polygon"/> 
      <rdfs:comment> 
This property returns a connected component of the interior boundary of a polygon. A polygon
can have zero or more iboundaryis properties 
      </rdfs:comment> 
   </rdf:Property> 

   <rdfs:Class rdf:ID="MultiPoint"> 
      <rdfs:subClassOf rdf:resource="#GeometryCollection"/> 
      <rdfs:comment> 
A MultiPoint is a 0 dimensional geometric collection. The elements of a MultiPoint are
restricted to Points. The points are not connected or ordered.  A MultiPoint is simple if no
two Points in the MultiPoint are equal (have identical coordinate values). The boundary of a
MultiPoint is the empty set. 
      </rdfs:comment> 
   </rdfs:Class> 

   <rdf:Property ID="pointMember"> 
      <rdfs:range rdf:resource="#Point"/> 
      <rdfs:domain rdf:resource="#MultiPoint"/> 
      <rdfs:comment> 
Returns the next point in a multipoint 
      </rdfs:comment> 
   </rdf:Property> 

   <rdfs:Class rdf:ID="MultiCurve"> 
      <rdfs:subClassOf rdf:resource="#GeometryCollection"/> 
      <rdfs:comment> 
A MultiCurve is a one-dimensional eometryCollection whose elements are Curves. MultiCurve is
present in this specification only to provide the context for the definition of a Multi-Line
String.  MultiCurve is simple if and only if all of its elements are simple, the only
intersections between any two elements occur at points that are on the boundary.  The boundary
of a MultiCurve is obtained by applying the 'mod 2' union rule: A point is in the boundary of a
MultiCurve if it is in the boundaries of an odd number of elements of the MultiCurve ([1],
section 3.12.3.2).  

MultiCurve is closed if all of its elements are closed. 

The boundary of a closed MultiCurve is always empty.  MultiCurve is defined as topologically
closed. 
      </rdfs:comment> 
   </rdfs:Class> 

   <rdfs:Class rdf:ID="MultiLineString"> 
      <rdfs:subClassOf rdf:resource="#GeometryCollection"/> 
      <rdfs:comment> 
A MultiLineString is a MultiCurve whose elements are LineStrings 
      </rdfs:comment> 
   </rdfs:Class> 

   <rdf:Property ID="lineStringMember"> 
      <rdfs:range rdf:resource="#LineString"/> 
      <rdfs:domain rdf:resource="#MultiLineString"/> 
      <rdfs:comment> 
Returns the next linestring in a multilinestring 
      </rdfs:comment> 
   </rdf:Property> 

   <rdfs:Class rdf:ID="MultiSurface"> 
      <rdfs:subClassOf rdf:resource="#GeometryCollection"/> 
      <rdfs:comment> 
Abstract class for complex 2-D geometries 
      </rdfs:comment> 
   </rdfs:Class> 

   <rdfs:Class rdf:ID="MultiPolygon"> 
      <rdfs:subClassOf rdf:resource="#MultiSurface"/> 
      <rdfs:comment> 
A MultiPolygon is a MultiSurface whose elements are Polygons. The assertions for MultiPolygons
are: 

1.  The interiors of 2 Polygons that are elements of a MultiPolygon may not intersect. 

2.  The Boundaries of any 2 Polygons that are elements of a MultiPolygon may not 'cross' and
may touch at only a finite number of points. (Note that crossing is prevented by assertion 1
above). 

3.  A MultiPolygon is defined as topologically closed. 

4.  A MultiPolygon may not have cut lines, spikes or punctures; a MultiPolygon is a Regular,
Closed point set: 

5.  The interior of a MultiPolygon with more than 1 Polygon is not connected, the number of
connected components of the interior of a MultiPolygon is equal to the number of Polygons in
the MultiPolygon. 

The boundary of a MultiPolygon is a set of closed curves (LinearRings) corresponding to the
boundaries of its element Polygons.  Each Curve in the boundary of the MultiPolygon is in the
boundary of exactly 1 element Polygon, and every Curve in the boundary of an element Polygon is
in the boundary of the MultiPolygon. 
      </rdfs:comment> 
   </rdfs:Class> 

   <rdf:Property ID="polygonMember"> 
      <rdfs:range rdf:resource="#Polygon"/> 
      <rdfs:domain rdf:resource="#MultiPolygon"/> 
      <rdfs:comment> 
Returns the next polygon in a multipolygon 
      </rdfs:comment> 
   </rdf:Property> 

<!--=================================================================================--> 
<!--============= This section defines the GML geometry properties. =================--> 
<!--========== All of these properties are sub-Properties of geometryproperty =======--> 
<!--=================================================================================--> 

   <rdf:Property ID="pointProperty"> 
      <rdfs:range rdf:resource="#Point"/> 
      <rdfs:subPropertyOf rdf:resource="#geometryProperty"/> 
      <rdfs:comment> 
Abstract property function that returns a point of the selected feature.  
      </rdfs:comment> 
   </rdf:Property> 

   <rdf:Property ID="lineStringProperty"> 
      <rdfs:range rdf:resource="#LineString"/> 
      <rdfs:subPropertyOf rdf:resource="#geometryProperty"/> 
      <rdfs:comment> 
Abstract property function that returns a linestring of the selected feature.  
      </rdfs:comment> 
   </rdf:Property> 

   <rdf:Property ID="polygonProperty"> 
      <rdfs:range rdf:resource="#Polygon"/> 
      <rdfs:subPropertyOf rdf:resource="#geometryProperty"/> 
      <rdfs:comment> 
Abstract property function that returns a polygon of the selected feature.  
      </rdfs:comment> 
   </rdf:Property> 

   <rdf:Property ID="location"> 
      <rdfs:subPropertyOf rdf:resource="#pointProperty"/> 
      <rdfs:comment> 
Returns a point of the selected feature.  
      </rdfs:comment> 
   </rdf:Property> 

   <rdf:Property ID="position"> 
      <rdfs:subPropertyOf rdf:resource="#pointProperty"/> 
      <rdfs:comment> 
Returns a point of the selected feature. 
      </rdfs:comment> 
   </rdf:Property> 

   <rdf:Property ID="centerOf"> 
      <rdfs:subPropertyOf rdf:resource="#pointProperty"/> 
      <rdfs:comment> 
Returns the center point of the selected feature. 
      </rdfs:comment> 
   </rdf:Property> 

   <rdf:Property ID="centerLineOf"> 
      <rdfs:subPropertyOf rdf:resource="#lineStringProperty"/> 
      <rdfs:comment> 
Returns a linestring which is the centerline of  the selected feature.  
      </rdfs:comment> 
   </rdf:Property> 

   <rdf:Property ID="edgeOf"> 
      <rdfs:subPropertyOf rdf:resource="#lineStringProperty"/> 
      <rdfs:comment> 
Returns a linestring which is an edge of the selected feature.  
      </rdfs:comment> 
   </rdf:Property> 

   <rdf:Property ID="extentOf"> 
      <rdfs:subPropertyOf rdf:resource="#polygonProperty"/> 
      <rdfs:comment> 
Returns a polygon which is the centerline of  the selected feature.  
      </rdfs:comment> 
   </rdf:Property> 

   <rdf:Property ID="coverage"> 
      <rdfs:subPropertyOf rdf:resource="#polygonProperty"/> 
      <rdfs:comment> 
Returns a polygon which is the centerline of  the selected feature.  
      </rdfs:comment> 
   </rdf:Property> 

   <rdf:Property ID="multiPointProperty"> 
      <rdfs:range rdf:resource="#MultiPoint"/> 
      <rdfs:subPropertyOf rdf:resource="#geometryProperty"/> 
      <rdfs:comment> 
Abstract property function that returns a multipoint of the selected feature.  
      </rdfs:comment> 
   </rdf:Property> 

   <rdf:Property ID="multiLineStringProperty"> 
      <rdfs:range rdf:resource="#MultiLineString"/> 
      <rdfs:subPropertyOf rdf:resource="#geometryProperty"/> 
      <rdfs:comment> 
Abstract property function that returns a multilinestring of the selected feature.  
      </rdfs:comment> 
   </rdf:Property> 

   <rdf:Property ID="multiPolygonProperty"> 
      <rdfs:range rdf:resource="#MultiPolygon"/> 
      <rdfs:subPropertyOf rdf:resource="#geometryProperty"/> 
      <rdfs:comment> 
Abstract property function that returns a MultiPolygon of the selected feature.  
      </rdfs:comment> 
   </rdf:Property> 

   <rdf:Property ID="multiLocation"> 
      <rdfs:subPropertyOf rdf:resource="#multiPointProperty"/> 
      <rdfs:comment> 
Returns a multipoint of the selected feature.  
      </rdfs:comment> 
   </rdf:Property> 

   <rdf:Property ID="multiPosition"> 
      <rdfs:subPropertyOf rdf:resource="#multiPointProperty"/> 
      <rdfs:comment> 
Returns a multipoint of the selected feature. 
      </rdfs:comment> 
   </rdf:Property> 

   <rdf:Property ID="multiCenterOf"> 
      <rdfs:subPropertyOf rdf:resource="#multiPointProperty"/> 
      <rdfs:comment> 
Returns the multi-center point of the selected feature. 
      </rdfs:comment> 
   </rdf:Property> 

   <rdf:Property ID="multiCenterLineOf"> 
      <rdfs:subPropertyOf rdf:resource="#multiLineStringProperty"/> 
      <rdfs:comment> 
Returns a multilinestring which is the multicenterline of  the selected feature.  
      </rdfs:comment> 
   </rdf:Property> 

   <rdf:Property ID="multiEdgeOf"> 
      <rdfs:subPropertyOf rdf:resource="#multiLineStringProperty"/> 
      <rdfs:comment> 
Returns a multilinestring which is a set of edges of the selected feature.  
      </rdfs:comment> 
   </rdf:Property> 

   <rdf:Property ID="multiExtentOf"> 
      <rdfs:subPropertyOf rdf:resource="#multiPolygonProperty"/> 
      <rdfs:comment> 
Returns a MultiPolygon which is the extent of  the selected feature.  
      </rdfs:comment> 
   </rdf:Property> 

   <rdf:Property ID="multiCoverage"> 
      <rdfs:subPropertyOf rdf:resource="#multiPolygonProperty"/> 
      <rdfs:comment> 
Returns a MultiPolygon which is the coverage of  the selected feature.  
      </rdfs:comment> 
   </rdf:Property> 
</rdf:RDF>
